\documentclass[a4paper,8pt,fleqn]{article}
\usepackage{amsmath}
\usepackage{amssymb}
\usepackage{multicol}
\usepackage{geometry}
\usepackage{titlesec}
\usepackage{fancyhdr}
\usepackage[T1]{fontenc} %Tillater bruk at norske bokstaver

% Geometry and layout
\geometry{a4paper, left=0.5in, right=0.5in, top=0.5in, bottom=0.5in}
\setlength{\columnsep}{1cm} % Column separation
\setlength{\parindent}{0pt} % No paragraph indentation

% Left aligned formulas
\setlength{\mathindent}{0pt} % No indentation for left-aligned formulas

% Define global font size commands (initially small)
\newcommand{\sectionfontsize}{\large}       % Font size for sections
\newcommand{\subsectionfontsize}{\small}   % Font size for subsections
\newcommand{\subsubsectionfontsize}{\small} % Font size for subsubsections
\newcommand{\bodyfontsize}{\small}         % Font size for body text
\newcommand{\mathfontsize}{\small}         % Font size for math

% Set the body font size (default without overwriting \normalsize)
\newcommand{\setbodyfontsize}{\bodyfontsize\selectfont}

% Global math sizes
\DeclareMathSizes{8}{8}{6}{5}

% Section formatting
\titleformat{\section}{\sectionfontsize\bfseries}{}{0.5em}{}
\titleformat{\subsection}{\subsectionfontsize\bfseries}{}{0.5em}{}
\titleformat{\subsubsection}{\subsubsectionfontsize\bfseries}{}{0.5em}{}

\titlespacing*{\section}{0pt}{1pt}{1pt} % Remove extra space around sections
\titlespacing*{\subsection}{0pt}{0.5pt}{0.5pt}
\titlespacing*{\subsubsection}{0pt}{0.5pt}{0.5pt}

% Disable section numbering globally
\setcounter{secnumdepth}{0}

% Custom footer
\pagestyle{fancy}
\fancyhf{}
\fancyfoot[C]{\scriptsize Matte 4000 - Per Erik Grønvik \hspace{1em} -- \hspace{1em} Page \thepage}

\begin{document}

% Apply body font size globally (without overwriting \normalsize)
\setbodyfontsize

% Multicolumn environment
\begin{multicols}{3}

\begin{minipage}{\linewidth}
% Title and class inside columns
{\bfseries Matte 400 Formula Sheet} \\
{\scriptsize Per Erik Grønvik \quad 2025}
\end{minipage}











\section{Separasjon av variabler}
\[
\frac{dy}{dx} = f(x)g(y)
\]
\[
\frac{1}{g(y)} \, dy = f(x) \, dx
\]
\[
\int \frac{1}{g(y)} \, dy = \int f(x) \, dx
\]

\section{Standardintegraler}
\subsection{Standardintegral for \(\frac{1}{a^2 - u^2}\)}
\[
\int \frac{1}{a^2 - u^2} \, du = \frac{1}{2a} \ln\left|\frac{a + u}{a - u}\right| + C
\]

\subsection{Standardintegral for \(\frac{1}{1 - u^2}\)}
\[
\int \frac{1}{1 - u^2} \, du = \text{artanh}(u) + C
\]

\subsection{Relasjon mellom \(\text{artanh}(x)\) og logaritmer}
\[
\text{artanh}(x) = \frac{1}{2} \ln\left(\frac{1 + x}{1 - x}\right)
\]

\subsection{Standardintegral for \(\frac{1}{a^2 - b^2x^2}\)}
\[
\int \frac{1}{a^2 - b^2x^2} \, dx = \frac{1}{2ab} \ln\left|\frac{a + bx}{a - bx}\right| + C
\]

\section{Generelle løsninger av lineære differensialligninger}
En lineær differensialligning på formen:
\[
\frac{dy}{dx} + P(x)y = Q(x)
\]
har den generelle løsningen:
\[
y(x) = e^{-\int P(x) \, dx} \left(\int Q(x) e^{\int P(x) \, dx} \, dx + C\right)
\]

\section{Eksponentiell vekst og logistisk vekst}
\subsection{Eksponentiell omskriving av logaritmer}
\[
\ln\left|\frac{a + u}{a - u}\right| = t + C \implies \frac{a + u}{a - u} = K e^{t}
\]

\subsection{Eksponentiell vekst eller forfall}
Differensialligningen:
\[
\frac{dy}{dt} = ky
\]
har løsningen:
\[
y(t) = Ce^{kt}
\]

\subsection{Logistisk vekst}
Differensialligningen:
\[
\frac{dy}{dt} = ky\left(1 - \frac{y}{M}\right)
\]
har løsningen:
\[
y(t) = \frac{M}{1 + Ce^{-kt}}
\]

\section{Trigonometriske substitusjoner}
Ved integrasjon av komplekse uttrykk kan trigonometriske substitusjoner forenkle prosessen:
\begin{itemize}
    \item For \(\sqrt{a^2 - x^2}\), bruk substitusjonen \(x = a \sin\theta\).
    \item For \(\sqrt{x^2 - a^2}\), bruk substitusjonen \(x = a \sec\theta\).
    \item For \(\sqrt{a^2 + x^2}\), bruk substitusjonen \(x = a \tan\theta\).
\end{itemize}






























\section*{Important Integrals}
\[
    \int_{-\infty}^\infty e^{-x^2} dx = \sqrt{\pi}.
    \]
\[
\int_{-\infty}^\infty e^{-a x^2} dx = \sqrt{\frac{\pi}{a}}, \quad a > 0.
\]
\[
\int_{-\infty}^\infty x^2 e^{-a x^2} dx = \sqrt{\frac{\pi}{a}} \cdot \frac{1}{2a}, \quad a > 0.
\]
\[
    \int_{-\infty}^\infty x^{2n} e^{-a x^2} dx = \sqrt{\frac{\pi}{a}} \cdot \frac{(2n-1)!!}{(2a)^n}, \quad n \in \mathbb{N}_0, \, a > 0,
    \]
\[
\int_a^b u v' \, dx = \big[ u v \big]_a^b - \int_a^b u' v \, dx
\]
\[
\int_a^b f(u) u' \, dx =\int_a^b f(u) \, \frac{du}{dx} dx = \int_{u(a)}^{u(b)} f(u) \, du
\]
\[
u = ax + b \Rightarrow \quad \frac{du}{dx} = a \Rightarrow \quad du = a \, dx \Rightarrow \quad dx = \frac{du}{a} 
\]




\section*{Important derivations and rules}

\[
\frac{d}{dx} f\big(g(x)\big) = f'\big(g(x)\big) \cdot g'(x).
\]
\[
\frac{d}{dx}\big(C \cdot f(x)\big) = C \cdot \frac{d}{dx}f(x),
\]





\textbf{Trigonometric functions} \\[-0.2cm]
\[
\int \cos(kx) dx = \frac{1}{k}\sin(kx) + C
\]
\[
\int \sin(kx) dx = -\frac{1}{k}\cos(kx) + C
\]
\[
\int \tan(x) dx = -ln\left|\cos(x)\right| + C
\]
\[
\int (1+\tan^2(x)) dx = \tan(x) + C
\]
\[
\int \frac{1}{\cos^2(x)} dx = \tan(x) +C
\]
\[
\int \sin^2(x) \, dx = -\frac{1}{4} \sin(2x) - \frac{x}{2} + C.
\]
\[
\int \cos^2(x) dx = \frac{1}{4}\sin(2x) + \frac{x}{2}+C
\]
\[
\int \tan^2(x) dx = \tan(x) - x + C
\]


\begin{minipage}{\linewidth}
\textbf{Sine and Cosine Powers and Products:}
\[
\sin^3(x) = \frac{3}{4}\sin(x) - \frac{1}{4}\sin(3x)
\]
\[
\sin(3x) = 3\sin(x) - 4\sin^3(x)
\]
\[
\cos(3x) = 4\cos^3(x) - 3\cos(x)
\]
\[
\sin^2(x) = \frac{1}{2} (1 - \cos(2x)) 
\]
\[
\cos^2(x)  = \frac{1}{2} (1 + \cos(2x))
\]

\[
\cos(2x) = \cos^2(x) - \sin^2(x) = 2\cos^2(x) - 1 = 1 - 2\sin^2(x)
\]

\[
\sin(2x) = 2\sin(x)\cos(x)
\]
\[
\tan(2x) = \frac{2\tan(x)}{1-\tan^2(x)}
\]
\end{minipage}
\begin{minipage}{\linewidth}
\textbf{Cotangent Definition:}
\[
\cot(\theta) = \frac{\cos(\theta)}{\sin(\theta)}
\]
\textbf{Addition formulas for cosine:}
\[
\cos(x + y) = \cos(x)\cos(y) - \sin(x)\sin(y)
\]
\[
\cos(x - y) = \cos(x)\cos(y) + \sin(x)\sin(y)
\]

\end{minipage}
\begin{minipage}{\linewidth}

\textbf{Partial Derivatives of a Function $f(x, y)$:} \\[-0.2cm]
\[
\frac{\partial f}{\partial x} \Bigg|_{x=x_0, y=y_0} = \lim_{h \to 0} \frac{f(x_0 + h, y_0) - f(x_0, y_0)}{h}
\]

\[
\frac{\partial f}{\partial y} \Bigg|_{x=x_0, y=y_0} = \lim_{h \to 0} \frac{f(x_0, y_0 + h) - f(x_0, y_0)}{h}
\]

\end{minipage}

\begin{minipage}{\linewidth}
\textbf{Euler's Formulas for Cosine and Sine:}
\[
\cos(x) = \frac{e^{ix} + e^{-ix}}{2}, \quad \sin(x) = \frac{e^{ix} - e^{-ix}}{2i}
\]
\end{minipage}

 \begin{minipage}{\linewidth}

\textbf{Euler's Formula} \\
\[
    e^{\pm ix} = \cos(x) \pm i \sin(x)
\]
Specific Forms of Euler's Formula (see +- syntax)
\[
    e^{-ix} = \cos(x) - i \sin(x)
\]
\[
    e^{ix} = \cos(x) + i \sin(x)
\]



\end{minipage}











\newpage
\section{Calculation rules compressed}


\begin{minipage}{\linewidth}
\subsection{Rules for complex konjugates}

\( z = a + bi \quad \Rightarrow \quad \overline{z} = a - bi \)\\
\( \overline{z_1 + z_2} \quad \Rightarrow \quad \overline{z_1} + \overline{z_2} \)\\
\( \overline{z_1 - z_2} \quad \Rightarrow \quad \overline{z_1} - \overline{z_2} \)\\
\( \overline{z_1 z_2} \quad \Rightarrow \quad \overline{z_1} \cdot \overline{z_2} \)\\
\( \overline{\frac{z_1}{z_2}} \quad \Rightarrow \quad \frac{\overline{z_1}}{\overline{z_2}}, \quad z_2 \neq 0 \)\\
\( z \in \mathbb{R} \quad \Rightarrow \quad \overline{z} = z \)\\
\( \overline{i} \quad \Rightarrow \quad -i \)\\
\( \overline{e^z} \quad \Rightarrow \quad e^{\overline{z}} \)\\
\( |\overline{z}| \quad \Rightarrow \quad |z| \)\\
\( \overline{\overline{z}} \quad \Rightarrow \quad z \)\\
\( \overline{\langle \psi, \phi \rangle} \quad \Rightarrow \quad \langle \phi, \psi \rangle \)\\


\end{minipage}
\begin{minipage}{\linewidth}

\subsection{Imaginary numbers}

\( i^2 = -1 \) \\ 
\( z = a + bi, \quad \text{where } a, b \in \mathbb{R} \) \\
\( |z| = \sqrt{a^2 + b^2} \) \\
\( \overline{z} = a - bi \) \\
\( z \cdot \overline{z} = |z|^2 = a^2 + b^2 \) \\
\( e^{i\theta} = \cos(\theta) + i\sin(\theta) \) \\
\( |e^{i\theta}| = 1 \) \\
\( \left(e^{i\theta}\right)^2 = e^{i(2\theta)} \) \\
\( z^n = 1 \implies z_k = e^{i\frac{2\pi k}{n}}, \quad k = 0, 1, 2, \dots, n-1 \) \\
\( z_1 = r_1 e^{i\theta_1}, \quad z_2 = r_2 e^{i\theta_2} \implies
z_1 \cdot z_2 = r_1 r_2 e^{i(\theta_1 + \theta_2)} \)
\( \frac{z_1}{z_2} = \frac{r_1}{r_2} e^{i(\theta_1 - \theta_2)} \) \\
\( \left(e^{i\theta}\right)^n = e^{i n \theta} = (\cos\theta + i\sin\theta)^n = \cos(n\theta) + i\sin(n\theta) \) \\
\end{minipage}


\begin{minipage}{\linewidth}
\subsection{Logarithmic Rules}
\(\log_b(xy) = \log_b(x) + \log_b(y)\) \\ 
\(\log_b\left(\frac{x}{y}\right) = \log_b(x) - \log_b(y)\) \\
\(\log_b(x^k) = k \cdot \log_b(x)\) \\
\(\log_b(1) = 0\) \\
\(\log_b(b) = 1\) \\
\(\log_b(x) = \frac{\ln(x)}{\ln(b)}\) \\
\(\ln(e^x) = x\) \\
\(\ln(1) = 0\) \\
\(\ln(ab) = \ln(a) + \ln(b)\) \\
\(\ln\left(\frac{a}{b}\right) = \ln(a) - \ln(b)\) \\
\(\ln(a^k) = k \cdot \ln(a)\)


\end{minipage}
\begin{minipage}{\linewidth}

\subsection{Rules for absolute value} 
\(|ab| = |a| \cdot |b|\)\\
\(\left| \frac{a}{b} \right| = \frac{|a|}{|b|}, \quad b \neq 0\)\\
\(|a + b| \leq |a| + |b|\)  (Trekantulikheten)\\
\(||a| - |b|| \leq |a - b|\)\\
\(||a|| = |a|\)\\
\(|a| = 0 \quad \Leftrightarrow \quad a = 0\)\\
\(|a|^2 = a^2\)\\
\(a(x) \in \mathbb{R}_{\geq 0} \implies |a(x)| = a(x)\)\\

\end{minipage}
\begin{minipage}{\linewidth}
\textbf{Rules for summation} 

\(\sum_{i=1}^n (a + b) = \sum_{i=1}^n a + \sum_{i=1}^n b\) \\
\(\sum_{i=1}^n c \cdot a_i = c \cdot \sum_{i=1}^n a_i, \quad \text{if } c \text{ is constant.}\) \\
\(\sum_{i=1}^n c = n \cdot c, \quad \text{if } c \text{ is constant.}\) \\
\(\sum_{i=1}^n (a_i \cdot b_i) \neq \left( \sum_{i=1}^n a_i \right) \cdot \left( \sum_{i=1}^n b_i \right), \quad \text{(not always equal!)}\) \\
\(\sum_{i=1}^n i = \frac{n(n+1)}{2}\) \\
\(\sum_{i=1}^n i^2 = \frac{n(n+1)(2n+1)}{6}\) \\
\(\sum_{i=1}^n (X_i - \bar{X}) X_i = \sum_{i=1}^n (X_i - \bar{X})^2\) \\
\(\sum_{i=1}^n (X_i - \bar{X})^2 = \sum_{i=1}^n X_i^2 - n\bar{X}^2\) \\
\(\sum_{i=1}^n (a X_i + b)^2 = a^2 \sum_{i=1}^n X_i^2 + 2ab \sum_{i=1}^n X_i + nb^2\) \\
\(\sum_{i=1}^n (x_i - \bar{x}) = 0\)
\(\bar{X} = \frac{1}{n} \sum_{i=1}^n X_i\)
\(\text{Cov}(X, Y) = \frac{1}{n} \sum_{i=1}^n (X_i - \bar{X})(Y_i - \bar{Y})\) \\
\(\text{Var}(X) = E(X^2) - E(X)^2\) \\
\end{minipage}


\begin{minipage}{\linewidth}
\textbf{Rules for expectation \(E\)} 
\(E(c) = c, \quad \text{if } c \text{ is constant.}\) \\
\(E(a + b) = E(a) + E(b)\) \\
\(E(c \cdot a) = c \cdot E(a), \quad \text{if } c \text{ is constant.}\) \\
\(E(a \cdot b) = E(a) \cdot E(b), \quad \text{if } a \text{ and } b \text{ are independent.}\) \\
\(E\left( \sum_{i=1}^n a_i \right) = \sum_{i=1}^n E(a_i)\) \\
\(E(a^2) = \text{Var}(a) + E(a)^2\) \\
\(E\left(\frac{a}{b}\right) \neq \frac{E(a)}{E(b)}, \quad \text{(not always equal, except in special cases).}\) \\
\(E(g(a)) = \int_{-\infty}^\infty g(x) f_a(x) \, dx, \quad \text{(for the continuous case with density function } f_a(x)\text{).}\) \\
\(E(g(a)) = \sum_{x} g(x) P(a = x), \quad \text{(for the discrete case).}\)
\end{minipage}


\newpage



\end{multicols}

\end{document}
